Additions to the replica model.
* PreparedCertificate's valid method now takes a SeqID
  for whcich we check if the PreparedCertificate is valid.
* LeaveView and SelectQuorumOfViewChangeMsgs send the newly
  created msgs right away.
* On leaving a View we check for PreparedCertificates in both
  the Working Window and in the latest View Change msg we have
  generated.

docs/sbft-formal-model/messages.dfy
@@ -40,10 +40,11 @@ module Messages {
     predicate WF() {
       (forall v | v in votes :: v.payload.Prepare?)
     }
-    predicate valid(quorumSize:nat) {
+    predicate valid(quorumSize:nat, seqID:SequenceID) {
       || empty()
       || (&& |votes| == quorumSize
           && WF()
+          && prototype().seqID == seqID
           && (forall v | v in votes :: v.payload == prototype()) // messages have to be votes that match eachother by the prototype 
           && UniqueSenders(votes))
     }
